SymDiff/Test/resilience/approx_feb_2015/examples/carbin-12/water-absHoudini/v1.bpl
@@ -1,0 +1,25 @@
+var FF: [int]int;
+var RS:[int]int;
+var K: int;
+
+  
+procedure water(len_FF: int, len_RS: int, N: int, gCUT2: int) returns ()
+{
+  var rand: int;
+  K := 1;
+
+  
+
+
+  while (K < N)
+  {
+      assert (K < len_FF);   
+      assert (K < len_RS);
+      if (RS[K] < gCUT2) {
+           //assert (K < len_FF); 
+           havoc rand;
+           FF[K] := rand;
+      }
+      K := K + 1;
+  }
+}
