SymDiff/Test/resilience/approx_feb_2015/examples/carbin-12/lu-absHoudini/ms_symdiff_file.bpl
@@ -1,0 +1,64 @@
+// Spec
+function {:inline true} MS$_v1.lu$_v2.lu(_v1.column: int, 
+    _v1.N: int, 
+    _v1.max_1: int, 
+    _v1.OK_old: bool, 
+    _v1.max: int, 
+    _v2.column: int, 
+    _v2.N: int, 
+    _v2.max_1: int, 
+    _v2.OK_old: bool, 
+    _v2.max: int)
+   : bool
+{
+  _v2.RelaxedEq(_v2.max, _v1.max) //manual
+}
+
+
+function {:existential true} __cand_pre_0(a:bool, b:bool):bool; 
+function {:existential true} __cand_post_0(a:bool, b:bool):bool; 
+
+
+function {:inline true} MS$_v1.lu_loop_anon5_LoopHead$_v2.lu_loop_anon5_LoopHead(_v1.in_column: int, 
+    _v1.in_N: int, 
+    _v1.in_max: int, 
+    _v1.in_i: int, 
+    _v1.in_a: int, 
+    _v1.OK_old: bool, 
+    _v1.out_max: int, 
+    _v1.out_i: int, 
+    _v1.out_a: int, 
+    _v2.in_column: int, 
+    _v2.in_N: int, 
+    _v2.in_max: int, 
+    _v2.in_i: int, 
+    _v2.in_a: int, 
+    _v2.in_old_a: int, 
+    _v2.OK_old: bool, 
+    _v2.out_max: int, 
+    _v2.out_i: int, 
+    _v2.out_a: int, 
+    _v2.out_old_a: int)
+   : bool
+{
+  __cand_post_0(_v2.out_max <= _v1.out_max + _v2.e, _v1.out_max <= _v2.out_max + _v2.e);
+}
+
+function {:inline true} MS_pre_$_v1.lu_loop_anon5_LoopHead$_v2.lu_loop_anon5_LoopHead(_v1.in_column: int, 
+    _v1.in_N: int, 
+    _v1.in_max: int, 
+    _v1.in_i: int, 
+    _v1.in_a: int, 
+    _v1.OK_old: bool, 
+    _v2.in_column: int, 
+    _v2.in_N: int, 
+    _v2.in_max: int, 
+    _v2.in_i: int, 
+    _v2.in_a: int, 
+    _v2.in_old_a: int, 
+    _v2.OK_old: bool)
+   : bool
+{
+  __cand_pre_0(_v2.in_max <= _v1.in_max + _v2.e, _v1.in_max <= _v2.in_max + _v2.e);
+}
+
